---
title: "cos(A)cos(B) = [cos(A-B) + cos(A+B)]/2"
categories: ["Trignometry", "Product-to-Sum Formulas"]


---



To derive the expression for $\cos A \cos B$, we can use Euler's formula, which states that $e^{i\theta} = \cos \theta + i \sin \theta$. By applying this to both angles $A$and$B$, we get:

$$e^{iA} = \cos A + i \sin A$$$$ e^{-iB} = \cos B - i \sin B$$Adding these equations, we obtain:$$e^{iA} + e^{-iB} = (\cos A + \cos B) + i(\sin A - \sin B)$$Similarly, subtracting these equations gives us:$$e^{iA} - e^{-iB} = (\cos A - \cos B) + i(\sin A + \sin B)$$By considering the sum of$e^{i(A+B)}$and$e^{-i(A-B)}$, we can use Euler's formula for exponentials:

$$e^{iA} + e^{-iB} = (\cos A + \cos B) + i(\sin A - \sin B)$$$$ e^{iB} + e^{-iA} = (\cos B + \cos A) + i(\sin B - \sin A)$$Adding these two results, we get:$$e^{iA} + e^{-iB} + e^{iB} + e^{-iA} = 2(\cos A + \cos B)$$This simplifies to:$$e^{i(A+B)} + e^{-i(A-B)} + e^{i(A-B)} + e^{-i(A+B)} = 4\cos A \cos B$$Dividing both sides by 4, we obtain:$$\cos A \cos B = \frac{1}{2} [\cos(A + B) + \cos(A - B)]$$Thus, the expression for$\cos A \cos B$is:$$\boxed{\frac{1}{2} [\cos(A + B) + \cos(A - B)]}$$
