---
title: "cos(A) - cos(B) = -2sin((A+B)/2)sin((A-B)/2)"
categories: ["Trignometry", "Sum-to-Product Formulas"]


---



To prove the identity $\cos A - \cos B = -2 \sin \left( \frac{A+B}{2} \right) \sin \left( \frac{A-B}{2} \right)$, we can use trigonometric identities and angle complement properties.

1. Express $\cos A$and$\cos B$as sines of complementary angles:$$\cos A = \sin\left(\frac{\pi}{2} - A\right) \quad \text{and} \quad \cos B = \sin\left(\frac{\pi}{2} - B\right)$$2. Use the identity for the difference of sines:$$\sin x - \sin y = 2 \cos\left( \frac{x + y}{2} \right) \sin\left( \frac{x - y}{2} \right)$$Let$x = \frac{\pi}{2} - A$and$y = \frac{\pi}{2} - B$.

3. Substitute these values into the sine difference identity:
   $$\sin\left(\frac{\pi}{2} - A\right) - \sin\left(\frac{\pi}{2} - B\right) = 2 \cos\left( \frac{(\frac{\pi}{2} - A) + (\frac{\pi}{2} - B)}{2} \right) \sin\left( \frac{(\frac{\pi}{2} - A) - (\frac{\pi}{2} - B)}{2} \right)$$4. Simplify the arguments:$$\cos\left( \frac{\pi - (A + B)}{2} \right) = \sin\left( \frac{A + B}{2} \right)$$$$\sin\left( \frac{(B - A)}{2} \right) = \sin\left( \frac{-(A - B)}{2} \right) = -\sin\left( \frac{A - B}{2} \right)$$5. Putting it all together:$$\cos A - \cos B = 2 \sin\left( \frac{A + B}{2} \right) (-\sin\left( \frac{A - B}{2} \right)) = -2 \sin\left( \frac{A + B}{2} \right) \sin\left( \frac{A - B}{2} \right)$$Thus, the identity is proven as:$$\boxed{\cos A - \cos B = -2 \sin \left( \frac{A+B}{2} \right) \sin \left( \frac{A-B}{2} \right)}$$
