---
title: "sin(A) - sin(B) = 2cos((A+B)/2)sin((A-B)/2)"
categories: ["Trignometry" , "Sum-to-Product Formulas"]


---



To prove the identity $\sin A - \sin B = 2\cos\left(\frac{A+B}{2}\right)\sin\left(\frac{A-B}{2}\right)$, we can use sum-to-product identities and angle addition formulas.

**Step-by-Step Explanation:**

1. **Express Sines Using Sum and Difference Formulas:**
   - Let $C = \frac{A + B}{2}$ and $D = \frac{A - B}{2}$.
   - Then, we can write:
     $$\sin A = \sin(C + D)$$$$\sin B = \sin(C - D)$$

2. **Expand Using Angle Addition Formulas:**
   - For $\sin(C + D)$:
     $$\sin(C + D) = \sin C \cos D + \cos C \sin D$$- For$ \sin(C - D) $:
     $$\sin(C - D) = \sin C \cos D - \cos C \sin D$$3. **Subtract the Two Expanded Sines:**$$\sin A - \sin B = [\sin C \cos D + \cos C \sin D] - [\sin C \cos D - \cos C \sin D]$$

4. **Simplify the Expression:**
   - Subtract term by term:
     $$(\sin C \cos D - \sin C \cos D) + (\cos C \sin D + \cos C \sin D)$$- This simplifies to:$$0 + 2\cos C \sin D = 2\cos C \sin D$$5. **Substitute Back$ C $and$ D $:**
   - Recall that $C = \frac{A + B}{2}$ and $D = \frac{A - B}{2}$.
   - Therefore:
     $$2\cos\left(\frac{A+B}{2}\right)\sin\left(\frac{A-B}{2}\right)$$

6. **Conclusion:**
   - Thus, we have shown that:
     $$\sin A - \sin B = 2\cos\left(\frac{A+B}{2}\right)\sin\left(\frac{A-B}{2}\right)$$
   
This completes the proof using sum-to-product identities and angle addition formulas.