---
title: "cos⁻¹(sin(x)) = x"
categories: ["Trignometry", "Composite Function Identities"]


---



To solve the equation $\cos y = \sin x$, we start by recognizing that $\sin x$can be rewritten using a trigonometric identity. Specifically, we know that:$$\sin x = \cos\left(\frac{\pi}{2} - x\right)$$Thus, the equation becomes:$$\cos y = \cos\left(\frac{\pi}{2} - x\right)$$This implies that$y$can be expressed as one of two angles within a periodic interval. The general solutions for$\cos \theta = \cos \phi$ are given by:

1. $\theta = \phi + 2k\pi$2.$\theta = -\phi + 2k\pi$

Applying this to our equation, we get two sets of solutions:

1. $y = \frac{\pi}{2} - x + 2k\pi$2.$y = x - \frac{\pi}{2} + 2k\pi$where$k$ is any integer.

Thus, the general solution to $\cos y = \sin x$is:$$\boxed{y = \frac{\pi}{2} - x + 2k\pi}$$and$$\boxed{y = x - \frac{\pi}{2} + 2k\pi}$$for any integer$k$.
