---
title: "sin²(θ/2) = (1 - cos(θ))/2"
tags: ["Trignometry" , "Half Angle Formulas"]
showTags: true
math: true
---



**Step-by-Step Proof**

We aim to prove the identity:

\[
\sin^{2}\left(\frac{\theta}{2}\right) = \frac{1 - \cos(\theta)}{2}
\]

**Step 1: Recall the Double-Angle Identity for Cosine**

The double-angle identity for cosine states that:

\[
\cos(2\alpha) = 1 - 2\sin^{2}(\alpha)
\]
Alternatively, it can also be written as:

\[
\cos(2\alpha) = 2\cos^{2}(\alpha) - 1
\]

**Step 2: Apply the Double-Angle Identity to \(\theta\) and \(2\theta/2\)**

Let’s consider a substitution where we set:

\[
\alpha = \frac{\theta}{2}
\]
Then, \(2\alpha = \theta\). Substituting into the double-angle identity:

**Using the first form (\( \cos(2\alpha) = 1 - 2\sin^{2}(\alpha) \)):**
\[
\cos(\theta) = 1 - 2\sin^{2}\left(\frac{\theta}{2}\right)
\]

**Step 3: Solve for \( \sin^{2}\left(\frac{\theta}{2}\right) \)**

Starting from the equation:

\[
\cos(\theta) = 1 - 2\sin^{2}\left(\frac{\theta}{2}\right)
\]
Subtract 1 from both sides:

\[
\cos(\theta) - 1 = -2\sin^{2}\left(\frac{\theta}{2}\right)
\]
Multiply both sides by \(-1\) to reverse the signs:

\[
1 - \cos(\theta) = 2\sin^{2}\left(\frac{\theta}{2}\right)
\]

**Step 4: Divide Both Sides by 2**

To isolate \( \sin^{2}\left(\frac{\theta}{2}\right) \), divide both sides of the equation by 2:

\[
\sin^{2}\left(\frac{\theta}{2}\right) = \frac{1 - \cos(\theta)}{2}
\]

**Conclusion**

Thus, we have proven that:

\[
\sin^{2}\left(\frac{\theta}{2}\right) = \frac{1 - \cos(\theta)}{2}
\]
This identity is known as the **squared half-angle identity for sine**, which relates the square of the sine of a half-angle to the cosine of the full angle.


