---
title: "csc⁻¹(-x) = -csc⁻¹(x)"
tags: ["Trignometry", "Negative Argument Relations"]
showTags: true
math: true
---



To determine the values of \( \csc^{-1}(1) \) and \( \csc^{-1}(-1) \):

1. Recall that \( \csc(\theta) = \frac{1}{\sin(\theta)} \). Therefore, \( \csc^{-1}(x) \) is the angle whose cosecant is \( x \).
2. The range of \( \csc^{-1}(x) \) is typically between \( -\pi/2 \) and \( \pi/2 \), excluding zero.
3. For \( x = 1 \):
   - \( \sin(\theta) = 1 \)
   - The angle whose sine is 1 is \( \pi/2 \).
   - Therefore, \( \csc^{-1}(1) = \pi/2 \).
4. For \( x = -1 \):
   - \( \sin(\theta) = -1 \)
   - The angle whose sine is -1 is \( -\pi/2 \).
   - Therefore, \( \csc^{-1}(-1) = -\pi/2 \).

Thus, the final answers are:

a) \boxed{\dfrac{\pi}{2}}  
b) \boxed{-\dfrac{\pi}{2}}
