---
title: "sin⁻¹(-x) = -sin⁻¹(x)"
tags: ["Trignometry", "Negative Argument Relations"]
showTags: true
math: true
---



To prove that \(\sin^{-1}(-x) = -\sin^{-1}(x)\), we start by understanding the definitions and properties of inverse trigonometric functions.

1. Let \(\alpha = \sin^{-1}(x)\). By definition, this means \(\sin(\alpha) = x\) and \(\alpha\) is within the range \([- \frac{\pi}{2}, \frac{\pi}{2}]\).
2. We need to find another angle \(\beta\) such that \(\sin(\beta) = -x\). Since \(\sin(-\theta) = -\sin(\theta)\), we can write \(\sin(-\alpha) = -x\).
3. The principal value of the inverse sine function, \(\sin^{-1}(y)\), is the angle in the range \([- \frac{\pi}{2}, \frac{\pi}{2}]\) such that \(\sin\) of that angle equals \(y\). Therefore, since \(-x = \sin(-\alpha)\), \(\beta\) must be equal to \(-\alpha\).
4. Thus, \(\sin^{-1}(-x) = -\alpha = -\sin^{-1}(x)\).

This holds true for all \(x\) within the principal domain of inverse sine, which is \([-1, 1]\). Therefore, we have shown that:

\[
\boxed{\sin^{-1}(-x) = -\sin^{-1}(x)}
\]
