---
title: "tan⁻¹(-x) = -tan⁻¹(x)"
tags: ["Trignometry", "Negative Argument Relations"]
showTags: true
math: true
---



To prove that \(\tan^{-1}(-x) = -\tan^{-1}(x)\), let's follow these steps:

**Step 1:** **Start with Definitions**

Let’s denote:
- Let \( y = \tan^{-1}(x) \). By definition, this means:
  \[
  \tan(y) = x
  \]
  
- Similarly, let \( z = \tan^{-1}(-x) \). This implies:
  \[
  \tan(z) = -x
  \]

**Step 2:** **Understand the Relationship Between \( y \) and \( z \)**

We need to find a relationship between \( y \) and \( z \).

From Step 1, we have:

\[
\tan(y) = x \quad \text{and} \quad \tan(z) = -x
\]
Notice that if \( \tan(z) = -x = -\tan(y) \), then there is a possible relationship between \( z \) and \( y \).

**Step 3:** **Consider the Tangent Function’s Periodicity**

The tangent function has a period of \( \pi \). This means:

\[
\tan(\theta + k\pi) = \tan\theta \quad \text{for any integer } k
\]
Given that:

\[
\tan(z) = -x = -\tan(y)
\]
and knowing that tangent is negative in the second and fourth quadrants, we can consider that \( z \) must be related to \( y \).

**Step 4:** **Determine the Specific Relationship**

Notice that:

\[
\tan(-y) = -\tan(y) = x
\]
But from Step 1, \( \tan(z) = -x \). Comparing this with the above, we have:

\[
\tan(z) = -\tan(y)
\]
Which implies:

\[
z = -y + k\pi \quad \text{for some integer } k
\]

**Step 5:** **Simplify Using Periodicity**

Since \( z = \tan^{-1}(-x) \), and we have established that \( z = -y \), substituting back:

\[
\tan^{-1}(-x) = -y
\]
But from Step 1, \( y = \tan^{-1}(x) \). Therefore:

\[
\tan^{-1}(-x) = -\tan^{-1}(x)
\]

**Conclusion:**

Thus, we have proven that:

\[
\tan^{-1}(-x) = -\tan^{-1}(x)
\]
This shows the relationship between the arctangent of a negative number and the negative of the arctangent of that positive number.
