---
title: "Multiplication: (a + bi)(c + di) = (ac - bd) + (ad + bc)i"
categories: ["Complex Numbers", "Operations"]
---



To multiply two complex numbers $(a + bi)$ and $(c + di)$, follow these steps:

1. **Distribute**: Multiply each term in the first complex number by each term in the second complex number:
   
$$
   (a + bi)(c + di) = ac + adi + bci + bdi^2
   $$


2. **Combine like terms**:
   - Real parts: $ac$
   - Imaginary parts: $adi + bci = (ad + bc)i$

3. **Remember that $i^2 = -1$**, substitute this into the equation:
   
$$
   ac + (ad + bc)i + bd(-1) = (ac - bd) + (ad + bc)i
   $$


4. **Final result**:
   
$$
   (a + bi)(c + di) = (ac - bd) + (ad + bc)i
   $$


Thus, the product of $(a + bi)$ and $(c + di)$ is $(ac - bd) + (ad + bc)i$.

**Summary**: By systematically applying the distributive property and remembering that $i^2 = -1$, you can multiply two complex numbers efficiently. This method ensures each term is accounted for correctly, leading to an accurate result.

\boxed{(a + bi)(c + di) = (ac - bd) + (ad + bc)i}
