---
title: "tan⁻¹(x) + cot⁻¹(x) = π/2"
categories: ["Trignometry", "Complementary Relations"]


---



To prove that $\tan^{-1}x + \cot^{-1}x = \frac{\pi}{2}$, we can use several approaches:

1. **Calculus Approach:**
   - Consider the function $f(x) = \tan^{-1}(x) + \cot^{-1}(x)$.
   - Compute the derivative $f'(x)$:
     $$f'(x) = \frac{1}{1 + x^2} - \frac{1}{1 + x^2} = 0$$- Since the derivative is zero,$f(x)$ is a constant function.
   - Evaluate $f(0)$:
     $$f(0) = \tan^{-1}(0) + \cot^{-1}(0) = 0 + \frac{\pi}{2} = \frac{\pi}{2}$$- Therefore, for all real numbers$x$, $f(x) = \frac{\pi}{2}$.

2. **Algebraic Approach:**
   - Let $\theta = \tan^{-1}(x)$. Then $x = \tan(\theta)$.
   - Since $\cot(\phi) = x$, we have $\phi = \cot^{-1}(x)$.
   - Note that $\cot(\phi) = \frac{1}{\tan(\phi)} = x$.
   - For any real $x$, it holds that:
     $$\theta + ( \frac{\pi}{2} - \theta ) = \frac{\pi}{2}$$- Therefore,$\tan^{-1}(x) + \cot^{-1}(x) = \frac{\pi}{2}$.

3. **Conclusion:**
   - Both the calculus and algebraic approaches confirm that $\tan^{-1}x + \cot^{-1}x$is a constant function equal to$\frac{\pi}{2}$.

Thus, the final answer is:

$$\boxed{\dfrac{\pi}{2}}$$
