---
title: "nC₀ + nC₁ + ... + nCₙ = 2ⁿ"
tags: ["Binomial Theorem", "Related Formulas"]
showTags: true
math: true
---



Sure! Let's explore the identity related to binomial coefficients and the sum \( C(n,0) + C(n,1) + \dotsb + C(n,n) = 2^n \). This will help us understand some key concepts in algebra and combinatorics.

### **Step-by-Step Explanation**

**1. Understanding Binomial Coefficients (\( C(n,k) \))**

Binomial coefficients are the coefficients of the terms in the expansion of the binomial expression \( (a + b)^n \). They represent the number of ways to choose \( k \) elements from a set of \( n \) distinct elements. Mathematically, they are given by:

\[
C(n,k) = \frac{n!}{k!(n - k)!}
\]

where:
- \( n! \) is the factorial of \( n \),
- \( k! \) is the factorial of \( k \),
- \( (n - k)! \) is the factorial of \( n - k \).

**2. The Sum \( C(n,0) + C(n,1) + \dotsb + C(n,n) = 2^n \)**

This identity states that when you sum all binomial coefficients from \( k = 0 \) to \( k = n \), the total is equal to \( 2^n \). Let's see why this is true.

**3. Combinatorial Interpretation**

Imagine a set of \( n \) distinct objects (like coins or people). We want to determine how many different subsets we can form from these objects, including the empty subset and the full set itself.

- **Subsets with 0 elements:** There's only **1** such subset—the empty set.
- **Subsets with 1 element:** There are \( C(n,1) \) ways to choose 1 object out of \( n \).
- **Subsets with 2 elements:** There are \( C(n,2) \) ways to choose 2 objects out of \( n \).
- ...
- **Subsets with \( k \) elements:** There are \( C(n,k) \) ways to choose \( k \) objects out of \( n \).

Since each subset can be formed in a unique way by choosing either an object or not for each element, the total number of subsets is:

\[
C(n,0) + C(n,1) + C(n,2) + \dotsb + C(n,n)
\]

This sum equals \( 2^n \) because each of the \( n \) objects can independently be either included or excluded from a subset. For each object, there are **2** choices (include or exclude), so for all \( n \) objects:

\[
2 \times 2 \times 2 \times \dotsb \times 2 = 2^n
\]

**4. Algebraic Proof Using the Binomial Theorem**

The binomial theorem states that:

\[
(a + b)^n = C(n,0)a^n b^0 + C(n,1)a^{n-1}b^1 + \dotsb + C(n,n)a^0b^n
\]

If we set \( a = 1 \) and \( b = 1 \), the expansion becomes:

\[
(1 + 1)^n = C(n,0)(1)^n (1)^0 + C(n,1)(1)^{n-1}(1)^1 + \dotsb + C(n,n)(1)^0(1)^n
\]

Simplifying each term, we have:

\[
2^n = C(n,0) + C(n,1) + C(n,2) + \dotsb + C(n,n)
\]

This algebraic proof confirms the identity.

**5. Example Calculation**

Let's verify this identity with a small value of \( n \).

- Let \( n = 3 \).
- Compute each binomial coefficient:
  - \( C(3,0) = 1 \)
  - \( C(3,1) = 3 \)
  - \( C(3,2) = 3 \)
  - \( C(3,3) = 1 \)
- Sum them up: \( 1 + 3 + 3 + 1 = 8 = 2^3 \)

This shows that the identity holds true for \( n = 3 \).

**6. General Proof Using Summation**

For a general proof, we can consider the sum:

\[
S = C(n,0) + C(n,1) + C(n,2) + \dotsb + C(n,n)
\]

We know that \( (1 + 1)^n = 2^n \). From the binomial theorem, this is equal to the expansion above. Therefore:

\[
S = (1 + 1)^n = 2^n
\]

This algebraic manipulation directly proves the identity.

### **Conclusion**

The identity \( C(n,0) + C(n,1) + \dotsb + C(n,n) = 2^n \) is fundamental in combinatorics and binomial expansions. It can be understood both through combinatorial reasoning (counting subsets) and algebraically using the binomial theorem.

**Final Answer:**

\[
C(n,0) + C(n,1) + \dotsb + C(n,n) = 2^n
\]
