---
title: "Relationships between consecutive terms"
tags: ["Binomial Theorem", "Related Formulas"]
showTags: true
math: true
---



The relationships between consecutive terms in the binomial expansion given by the binomial theorem can be derived using the general term formula:

\[
T_k = C(n, k) \cdot a^{n - k} \cdot b^k
\]

For each pair of consecutive terms \( T_k \) and \( T_{k+1} \), we can express their ratio as follows:

1. **Express the Ratio:**
   \[
   \frac{T_{k+1}}{T_k} = \frac{C(n, k + 1) \cdot a^{n - (k + 1)} \cdot b^{k + 1}}{C(n, k) \cdot a^{n - k} \cdot b^k}
   \]

2. **Simplify Binomial Coefficients:**
   Using the properties of combinations:
   \[
   C(n, k + 1) = C(n, k) \cdot \frac{n - k}{k + 1}
   \]

3. **Substitute and Simplify Exponents:**
   \[
   \frac{T_{k+1}}{T_k} = \left( \frac{n - k}{k + 1} \right) \cdot \left( \frac{b}{a} \right)
   \]

4. **Express Each Term in Terms of the Previous One:**
   \[
   T_{k+1} = T_k \cdot \left( \frac{n - k}{k + 1} \right) \cdot \left( \frac{b}{a} \right)
   \]

**Conclusion:**

Each consecutive term in the binomial expansion can be obtained by multiplying the previous term by the factor \( \left( \frac{n - k}{k + 1} \right) \cdot \left( \frac{b}{a} \right) \). This relationship allows one to compute each term based on its predecessor, illustrating how terms progress within the expansion. 

**Example:**

For \( n = 4 \), \( a = x \), and \( b = y \):

- **Term_0:** \( T_0 = x^4 \)
- **Term_1:** \( T_1 = T_0 \cdot \frac{4 - 0}{0 + 1} \cdot \frac{y}{x} = 4x^3y \)
- **Term_2:** \( T_2 = T_1 \cdot \frac{4 - 1}{1 + 1} \cdot \frac{y}{x} = 6x^2y^2 \)

This demonstrates the application of the derived relationship.
