---
title: "cos(-θ) = cos(θ)"
tags: ["Trignometry", "Even/Odd Properties"]
showTags: true
math: true
---



**Step-by-Step Proof of \(\cos(-\theta) = \cos(\theta)\)**

1. **Understand Cosine on the Unit Circle:**
   - Consider a unit circle (a circle with radius \(r = 1\)) centered at the origin of a coordinate system.
   - For an angle \(\theta\), a point \(P\) on the unit circle is represented as \((x, y)\).
   - By definition:
     \[
     x = \cos(\theta) \quad \text{and} \quad y = \sin(\theta)
     \]
   
2. **Reflecting an Angle by \(-\theta\):**
   - A negative angle \(-\theta\) represents a rotation in the clockwise direction instead of counterclockwise.
   - The point corresponding to \(-\theta\) is also on the unit circle, but it's located at \( (x, -y) \).
   
3. **Expressing \(\cos(-\theta)\):**
   - For the angle \(-\theta\), the x-coordinate of the corresponding point is still \(x\):
     \[
     \cos(-\theta) = x
     \]
   - Since \(x = \cos(\theta)\), we substitute:
     \[
     \cos(-\theta) = \cos(\theta)
     \]
   
4. **Conclusion:**
   - The equality \(\cos(-\theta) = \cos(\theta)\) holds true because the cosine function is an even function, symmetric about the y-axis.
   - This means that for any angle \(\theta\), its cosine value is the same as the cosine of its negative counterpart.

**Final Answer:**
\[
\boxed{\cos(-\theta) = \cos(\theta)}
\]
