---
title: "cot(-θ) = -cot(θ)"
tags: ["Trignometry", "Even/Odd Properties"]
showTags: true
math: true
---



To prove that \(\cot(-\theta) = -\cot(\theta)\), we'll use the definitions of the trigonometric functions and their properties.

**Step 1: Understand the Definition of Cotangent**

The cotangent function is defined as:

\[
\cot(\theta) = \frac{\cos(\theta)}{\sin(\theta)}
\]

**Step 2: Apply Negative Angle Identities to Cosine and Sine**

We know that cosine is an even function, meaning:

\[
\cos(-\theta) = \cos(\theta)
\]
And sine is an odd function, meaning:

\[
\sin(-\theta) = -\sin(\theta)
\]

**Step 3: Compute cot(-θ)**

Using the definitions and identities from Steps 1 and 2:

\[
\cot(-\theta) = \frac{\cos(-\theta)}{\sin(-\theta)} = \frac{\cos(\theta)}{-\sin(\theta)} = -\frac{\cos(\theta)}{\sin(\theta)} = -\cot(\theta)
\]

**Conclusion**

Therefore, we've shown that:

\[
\boxed{\cot(-\theta) = -\cot(\theta)}
\]
