---
title: "tan(-θ) = -tan(θ)"
tags: ["Trignometry" ,"Even/Odd Properties"]
showTags: true
math: true
---



Let's provide a clear, step-by-step proof of the identity \(\tan(-\theta) = -\tan(\theta)\).

**Step 1: Understand the Definition of Tangent**

The tangent function is defined as:

\[
\tan(\theta) = \frac{\sin(\theta)}{\cos(\theta)}
\]
Similarly, for a negative angle \( -\theta \), we have:

\[
\tan(-\theta) = \frac{\sin(-\theta)}{\cos(-\theta)}
\]

**Step 2: Use the Odd-Even Properties of Sine and Cosine**

The sine function is **odd**, which means:

\[
\sin(-\theta) = -\sin(\theta)
\]
The cosine function is **even**, so:

\[
\cos(-\theta) = \cos(\theta)
\]

**Step 3: Substitute the Odd and Even Properties into the Tangent Function**

Using the above properties, we substitute in the expression for \(\tan(-\theta)\):

\[
\tan(-\theta) = \frac{\sin(-\theta)}{\cos(-\theta)} = \frac{-\sin(\theta)}{\cos(\theta)}
\]

**Step 4: Simplify the Expression**

The numerator is \(-\sin(\theta)\), and the denominator is \(\cos(\theta)\):

\[
\tan(-\theta) = -\frac{\sin(\theta)}{\cos(\theta)} = -\tan(\theta)
\]
Thus, we have shown that:

\[
\tan(-\theta) = -\tan(\theta)
\]

**Conclusion**

By applying the properties of odd and even functions to the sine and cosine components in the tangent function's definition, we've proven that \(\tan(-\theta)\) is indeed equal to \(-\tan(\theta)\).