---
title: "Expansion of (x + 1/x)‚Åø"
categories: ["Binomial Theorem", "Special Cases and Forms"]


---



The binomial expansion of $(x + 1/x)^n$results in terms where each term can be expressed as:$$(x + 1/x)^n = \sum_{k=0}^{n} C(n,k) x^{n - k} \cdot (1/x)^k$$Simplifying, each term becomes:$$C(n,k) x^{n - 2k}$$This results in a sum of terms where the exponents are$n, n-2, n-4, \ldots, -n$, all multiples of 2. The coefficients are given by the binomial coefficients $C(n,k)$.

### Detailed Steps:

1. **Apply Binomial Theorem**: Start with the expansion $(x + y)^n = \sum_{k=0}^{n} C(n,k) x^{n - k} y^k$.

2. **Substitute $y$with$1/x$**: Replace $y$with$1/x$to get$(x + 1/x)^n = \sum_{k=0}^{n} C(n,k) x^{n - k} (1/x)^k$.

3. **Simplify Each Term**: Simplify each term as:
   $$C(n,k) x^{n - k} \cdot (1/x)^k = C(n,k) x^{n - 2k}$$4. **Identify Exponents**: The exponents of$x$in each term are$n, n-2, n-4, \ldots, -n$, all multiples of 2.

5. **Coefficient Structure**: Each coefficient is a binomial coefficient from the expansion, ensuring positive values.

6. **Examples for Clarity**:
   - For $n=1$: $(x + 1/x)^1 = x + 1/x$- For$n=2$: $(x + 1/x)^2 = x^2 + 2 + 1/x^2$- For$n=3$: $(x + 1/x)^3 = x^3 + 3x + 3/x + 1/x^3$- For$n=4$: $(x + 1/x)^4 = x^4 + 4x^2 + 6 + 4/x^2 + 1/x^4$

### Conclusion:

The expansion of $(x + 1/x)^n$is a sum of terms where each term has an exponent that is a multiple of 2, starting from$n$and decreasing by 2 until reaching$-n$. The coefficients are binomial coefficients, ensuring all terms have positive values. This pattern holds regardless of whether $n$ is even or odd, with the exponents always maintaining consistency in their structure.
