---
title: "(x - 1)‚Åø expansion"
categories: ["Binomial Theorem", "Special Cases and Forms"]


---



The expansion of $(x - 1)^n$can be written using the binomial theorem, which states:$$(x + y)^n = \sum_{k=0}^{n} C(n,k) x^{n-k} y^k$$In our case,$y = -1$, so substituting we get:

$$(x - 1)^n = \sum_{k=0}^{n} C(n,k) x^{n - k} (-1)^k$$This simplifies to:$$\sum_{k=0}^{n} (-1)^k C(n, k) x^{n - k}$$The expansion is a sum of terms where each term is given by$(-1)^k$multiplied by the binomial coefficient$C(n,k)$, with the power of $x$decreasing from$n$to$0$. The sign alternates for each subsequent term because of the factor $(-1)^k$.

For example, when $n = 3$:

$$(x - 1)^3 = x^3 - 3x^2 + 3x - 1$$

This expansion is a sum of terms where:

- The first term is $C(3,0) (-1)^0 x^{3} = x^3$- The second term is$- C(3,1) (-1)^1 x^{2} = -3x^2$- The third term is$+ C(3,2) (-1)^2 x^{1} = +3x$- The fourth term is$- C(3,3) (-1)^3 = -1$Thus, the expansion is:$$(x - 1)^n = \sum_{k=0}^{n} (-1)^k C(n,k) x^{n - k}$$
