---
title: "cot⁻¹(-x) = π - cot⁻¹(x)"
categories: ["Trignometry", "Negative Argument Relations"]


---



**Step-by-Step Explanation and Proof:**

We aim to prove the following identity:

$$\cot^{-1}(-x) = \pi - \cot^{-1}(x)$$**Step 1:** Let’s define a variable$ y $such that:$$y = \cot^{-1}(x)$$This means that:$$x = \cot(y)$$Since$ \cot(\theta) = \frac{1}{\tan(\theta)} $, we can also write:

$$x = \frac{1}{\tan(y)}$$**Step 2:** Substitute$ x $into the original equation. We have:$$\cot^{-1}(-x) = \pi - y$$But since$ x = \frac{1}{\tan(y)} $, substitute this in:

$$\cot^{-1}\left(-\frac{1}{\tan(y)}\right) = \pi - y$$**Step 3:** Simplify the left side. Recognize that:$$-\frac{1}{\tan(y)} = \tan\left(\frac{\pi}{2} - y\right)$$So, we can rewrite the equation as:$$\cot^{-1}\left(\tan\left(\frac{\pi}{2} - y\right)\right) = \pi - y$$**Step 4:** Recall that$ \cot^{-1}(z) + \tan^{-1}(z) = \frac{\pi}{2} $for any real number$ z $. However, in this case, since we have a negative inside the cotangent inverse, we adjust accordingly.

**Step 5:** Since:

$$\tan\left(\frac{\pi}{2} - y\right) = \cot(y)$$Taking the reciprocal of both sides (since$ x = \cot(y) $):

$$\cot\left(\frac{\pi}{2} - y\right) = \tan(y)$$**Step 6:** Now, take the cotangent inverse on both sides:$$\frac{\pi}{2} - y = \cot^{-1}\left(\tan(y)\right)$$But$ \tan(y) = x $, so:

$$\frac{\pi}{2} - y = \cot^{-1}(x)$$**Step 7:** Solve for$ y $:

$$y = \frac{\pi}{2} - \cot^{-1}(x)$$Recall that$ y = \cot^{-1}(x) $, so:

$$\cot^{-1}(x) = \frac{\pi}{2} - \cot^{-1}\left(-x\right)$$**Step 8:** Rearranging the equation gives us:$$\cot^{-1}(-x) = \pi - \cot^{-1}(x)$$This completes the proof.$$\boxed{\cot^{-1}(-x) = \pi - \cot^{-1}(x)}$$
