---
title: "tan(2θ) = 2tan(θ)/(1 - tan²(θ))"
categories: ["Trignometry", "Double Angle Formulas"]
---


**Step-by-Step Proof of $\tan(2\theta) = \frac{2\tan(\theta)}{1 - \tan^2(\theta)}$**

We aim to prove the double-angle identity for tangent:

$$\tan(2\theta) = \frac{2\tan(\theta)}{1 - \tan^2(\theta)}$$

**Recall the Tangent Addition Formula**

The tangent of a sum of two angles is given by:

$$\tan(a + b) = \frac{\tan a + \tan b}{1 - \tan a \tan b}$$where$a$and$b$ are any real numbers for which the denominator is not zero.

**Apply the Addition Formula to $\tan(2\theta)$**

Let’s set both angles equal to $\theta$:

$$\tan(2\theta) = \tan(\theta + \theta)$$Using the addition formula:$$\tan(2\theta) = \frac{\tan \theta + \tan \theta}{1 - (\tan \theta)(\tan \theta)}$$

**Simplify the Expression**

Simplify both the numerator and the denominator:

- **Numerator:**
$$\tan \theta + \tan \theta = 2\tan \theta$$- **Denominator:**$$1 - (\tan \theta)(\tan \theta) = 1 - \tan^2(\theta)$$

**Combine the Results**

Putting it all together:

$$\tan(2\theta) = \frac{2\tan \theta}{1 - \tan^2 \theta}$$Thus, we have proven that:$$\tan(2\theta) = \frac{2\tan(\theta)}{1 - \tan^2(\theta)}$$

This completes the proof of the double-angle identity for tangent.
