---
title: "sin(A) + sin(B) = 2sin((A+B)/2)cos((A-B)/2)"
tags: ["Trignometry" , "Sum-to-Product Formulas"]
showTags: true
math: true
---



**Step-by-Step Explanation and Proof**

We aim to prove the trigonometric identity:

\[
\sin(A) + \sin(B) = 2\sin\left(\frac{A+B}{2}\right)\cos\left(\frac{A-B}{2}\right)
\]

**1. Recall the Sum-to-Product Identity for Sines**

One of the sum-to-product identities in trigonometry is:

\[
\sin(x) + \sin(y) = 2\sin\left(\frac{x+y}{2}\right)\cos\left(\frac{x-y}{2}\right)
\]

**2. Substitute Variables with \(A\) and \(B\)**

Letâ€™s substitute \(x = A\) and \(y = B\) into the identity:

\[
\sin(A) + \sin(B) = 2\sin\left(\frac{A+B}{2}\right)\cos\left(\frac{A-B}{2}\right)
\]

**3. Conclusion**

After substitution, we directly obtain the desired identity:

\[
\boxed{\sin(A) + \sin(B) = 2\sin\left(\frac{A+B}{2}\right)\cos\left(\frac{A-B}{2}\right)}
\]

Thus, by applying the sum-to-product identity for sine functions, we have proven that:

\[
\sin(A) + \sin(B) = 2\sin\left(\frac{A+B}{2}\right)\cos\left(\frac{A-B}{2}\right)
\]
