---
title: "cos⁻¹(x) = π/2 - sin⁻¹(x)"
tags: ["Trignometry", "Pythagorean Identities"]
showTags: true
math: true
---



To prove that \(\cos^{-1}(x) = \frac{\pi}{2} - \sin^{-1}(x)\), we can use trigonometric identities and properties of inverse functions.

**Step-by-Step Explanation:**

1. **Let \(\alpha = \sin^{-1}(x)\):**
   - By definition, this means \(\sin(\alpha) = x\).

2. **Apply the co-function identity:**
   - We know that \(\cos\left(\frac{\pi}{2} - \alpha\right) = \sin(\alpha)\).
   - Substituting \(\sin(\alpha) = x\) gives \(\cos\left(\frac{\pi}{2} - \alpha\right) = x\).

3. **Interpret the result:**
   - Since \(\cos^{-1}(x)\) is the angle whose cosine is \(x\), and it yields values in the range \([0, \pi]\).
   - Therefore, \(\frac{\pi}{2} - \alpha = \cos^{-1}(x)\).

4. **Substitute back for \(\alpha\):**
   - Since \(\alpha = \sin^{-1}(x)\), we have \(\cos^{-1}(x) = \frac{\pi}{2} - \sin^{-1}(x)\).

Thus, the identity is proven:

\[
\cos^{-1}(x) = \frac{\pi}{2} - \sin^{-1}(x)
\]
