---
title: "sin θ = 1/csc θ and csc θ = 1/sin θ"
tags: ["Trignometry", "Reciprocal Identities"]
showTags: true
math: true
---



To prove that \(\sin \theta = \frac{1}{\csc \theta}\) and \(\csc \theta = \frac{1}{\sin \theta}\), let's proceed step by step.

**Step 1: Understand the Definitions**

- **Sine Function (\(\sin \theta\))**: In a right triangle, it represents the ratio of the length of the side opposite to an angle θ (relative to the hypotenuse).

- **Cosecant Function (\(\csc \theta\))**: It is defined as the reciprocal of the sine function. Specifically:
  \[
  \csc \theta = \frac{1}{\sin \theta}
  \]

**Step 2: Prove \(\sin \theta = \frac{1}{\csc \theta}\)**

- Starting with the definition of cosecant:
  \[
  \csc \theta = \frac{1}{\sin \theta}
  \]
  
- To find \(\sin \theta\) in terms of \(\csc \theta\), take the reciprocal of both sides:
  \[
  \sin \theta = \frac{1}{\csc \theta}
  \]
  
**Conclusion**: 
\[
\sin \theta = \frac{1}{\csc \theta} \quad \text{and} \quad \csc \theta = \frac{1}{\sin \theta}
\]

This completes the proof of both equalities.
