---
title: "sec(π/2 - θ) = csc(θ)"
tags: ["Trignometry", "Cofunction Identities"]
showTags: true
math: true
---



To prove that \(\sec\left(\frac{\pi}{2} - \theta\right) = \csc\theta\), follow these steps:

**Step 1: Understand the Definitions**

- **Secant Function:** The secant of an angle is the reciprocal of the cosine function. Mathematically,
  
  \[
  \sec x = \frac{1}{\cos x}
  \]

- **Cosecant Function:** The cosecant of an angle is the reciprocal of the sine function. Mathematically,

  \[
  \csc x = \frac{1}{\sin x}
  \]

**Step 2: Express secant as a Reciprocal**

Start with the left-hand side (LHS) of the equation:

\[
\sec\left(\frac{\pi}{2} - \theta\right) = \frac{1}{\cos\left(\frac{\pi}{2} - \theta\right)}
\]

**Step 3: Use a Co-Function Identity**

Recall that:

\[
\cos\left(\frac{\pi}{2} - \theta\right) = \sin\theta
\]

This identity is known as the co-function identity. Substitute this into the equation from Step 2:

\[
\sec\left(\frac{\pi}{2} - \theta\right) = \frac{1}{\sin\theta}
\]

**Step 4: Compare to Cosecant**

Notice that:

\[
\frac{1}{\sin\theta} = \csc\theta
\]

Therefore,

\[
\sec\left(\frac{\pi}{2} - \theta\right) = \csc\theta
\]

**Conclusion:**

We have shown through the definitions and co-function identities that:

\[
\sec\left(\frac{\pi}{2} - \theta\right) = \csc\theta
\]

This completes the proof.
