---
title: "tan²θ + 1 = sec²θ"
categories: ["Trignometry", "Pythagorean Identities"]


---



 Let's break down the proof step by step.

**Given**:  
We want to show that $\tan^{2}(\theta) + 1 = \sec^{2}(\theta)$.

**Step 1**: Express $\tan(\theta)$in terms of sine and cosine.$$\tan(\theta) = \frac{\sin(\theta)}{\cos(\theta)}$$**Step 2**: Square both sides to get$\tan^{2}(\theta)$.  
$$\tan^{2}(\theta) = \left(\frac{\sin(\theta)}{\cos(\theta)}\right)^{2} = \frac{\sin^{2}(\theta)}{\cos^{2}(\theta)}$$**Step 3**: Add 1 to both sides of the equation.$$\tan^{2}(\theta) + 1 = \frac{\sin^{2}(\theta)}{\cos^{2}(\theta)} + 1$$**Step 4**: Express 1 as a fraction with the same denominator as$\tan^{2}(\theta)$.  
$$1 = \frac{\cos^{2}(\theta)}{\cos^{2}(\theta)}$$**Step 5**: Combine the two fractions on the right side.$$\tan^{2}(\theta) + 1 = \frac{\sin^{2}(\theta) + \cos^{2}(\theta)}{\cos^{2}(\theta)}$$**Step 6**: Use the Pythagorean identity$\sin^{2}(\theta) + \cos^{2}(\theta) = 1$.  
$$\tan^{2}(\theta) + 1 = \frac{1}{\cos^{2}(\theta)}$$**Step 7**: Recognize that$\frac{1}{\cos(\theta)} = \sec(\theta)$, so squaring both sides gives:  
$$\left(\frac{1}{\cos(\theta)}\right)^{2} = \frac{1}{\cos^{2}(\theta)}$$**Step 8**: Therefore,$$\tan^{2}(\theta) + 1 = \sec^{2}(\theta)$$This completes the proof that$\tan^{2}(\theta) + 1$equals$\sec^{2}(\theta)$.