---
title: "csc(csc⁻¹(x)) = x, for |x| ≥ 1"
tags: ["Trignometry","Basic Inverse Relations"]
showTags: true
math: true
---



To prove that \(\csc(\csc^{-1}(x)) = x\) for \(|x| \geq 1\), we start by understanding the definitions and properties of inverse trigonometric functions.

1. Let \(\theta = \csc^{-1}(x)\). By definition, this implies that \(\csc(\theta) = x\).
2. We need to compute \(\csc(\csc^{-1}(x))\), which is equivalent to finding \(\csc(\theta)\).
3. Since \(\theta\) is defined such that \(\csc(\theta) = x\), substituting back, we get \(\csc(\csc^{-1}(x)) = x\).

This proof relies on the understanding that applying a function after its inverse cancels out, provided they are within their respective domains and ranges. For \(\csc^{-1}(x)\), \(|x|\) must be at least 1 to ensure the angle is valid.

Thus, the detailed step-by-step proof confirms that:

\[
\boxed{x}
\]
